LeanLR/ProgramLogics/LogRel.lean
@@ -4,3 +4,5 @@ import LeanLR.ProgramLogics.LogRel.Syntactic
 import LeanLR.ProgramLogics.LogRel.GhostStateLib
 import LeanLR.ProgramLogics.LogRel.GhostState
 import LeanLR.ProgramLogics.LogRel.LogRel
+import LeanLR.ProgramLogics.LogRel.Adequacy
+import LeanLR.ProgramLogics.LogRel.Examples
